code/ecdsap256/dist/Hacl_P256.h
@@ -56,6 +56,25 @@ Hacl_P256_ecdsa_sign_p256_sha2_ladder(
 );
 
 /*
+ Input: result buffer: uint8[64], 
+ m buffer: uint8 [mLen], 
+ priv(ate)Key: uint8[32], 
+ k (nonce): uint32[32]. 
+  
+ Output: bool, where True stands for the correct signature generation. False value means that an error has occurred. 
+  
+ The private key and the nonce are expected to be more than 0 and less than the curve order.
+*/
+bool
+Hacl_P256_ecdsa_sign_p256_sha2_comb(
+  uint8_t *result,
+  uint32_t mLen,
+  uint8_t *m,
+  uint8_t *privKey,
+  uint8_t *k
+);
+
+/*
  The input of the function is considered to be public, 
   thus this code is not secret independent with respect to the operations done over the input.
   
@@ -68,6 +87,26 @@ Hacl_P256_ecdsa_sign_p256_sha2_ladder(
 */
 bool
 Hacl_P256_ecdsa_verif_p256_sha2_ladder(
+  uint32_t mLen,
+  uint8_t *m,
+  uint8_t *pubKey,
+  uint8_t *r,
+  uint8_t *s
+);
+
+/*
+ The input of the function is considered to be public, 
+  thus this code is not secret independent with respect to the operations done over the input.
+  
+ Input: m buffer: uint8 [mLen], 
+ pub(lic)Key: uint8[64], 
+ r: uint8[32], 
+ s: uint8[32]. 
+  
+ Output: bool, where true stands for the correct signature verification. 
+*/
+bool
+Hacl_P256_ecdsa_verif_p256_sha2_comb_radix(
   uint32_t mLen,
   uint8_t *m,
   uint8_t *pubKey,
